compiler/backend/semantics/closPropsScript.sml
@@ -1873,6 +1873,7 @@ val ssgc_free_def = Define`
     (∀n m e. FLOOKUP s.code n = SOME (m,e) ⇒ set_globals e = {||}) ∧
     (∀n vl. FLOOKUP s.refs n = SOME (ValueArray vl) ⇒ EVERY vsgc_free vl) ∧
     (∀v. MEM (SOME v) s.globals ⇒ vsgc_free v) ∧
+    (∀v. s.mutable_global = SOME v ⇒ vsgc_free v) ∧
     (∀n exp aux. SND (s.compile_oracle n) = (exp, aux) ⇒ EVERY esgc_free exp ∧
          elist_globals (MAP (SND o SND) aux) = {||})
 `;
